Garden/OpenVM/BranchEq/core.v
@@ -1,830 +1,215 @@
-Require Import ZArith.
-Require Import List.
-Import ListNotations.
+Require Import Garden.Plonky3.M.
+Require Import Garden.Plonky3.MExpr.
 
-(* 
-use std::{
-    array,
-    borrow::{Borrow, BorrowMut},
-};
-
-use openvm_circuit::arch::{
-    AdapterAirContext, AdapterRuntimeContext, ImmInstruction, Result, VmAdapterInterface,
-    VmCoreAir, VmCoreChip,
-};
-use openvm_circuit_primitives::utils::not;
-use openvm_circuit_primitives_derive::AlignedBorrow;
-use openvm_instructions::{instruction::Instruction, LocalOpcode};
-use openvm_rv32im_transpiler::BranchEqualOpcode;
-use openvm_stark_backend::{
-    interaction::InteractionBuilder,
-    p3_air::{AirBuilder, BaseAir},
-    p3_field::{Field, FieldAlgebra, PrimeField32},
-    rap::BaseAirWithPublicValues,
-};
-use serde::{Deserialize, Serialize};
-use serde_big_array::BigArray;
-use strum::IntoEnumIterator;
-*)
-
-(* ****TOOLS**** *)
-(* Just a modified product type to conviniently record the constraints.
-Writer monad is definitely better but I feel it too heavy to implement for now
-*)
-Definition RecordRun {A B : Set} : Type := A * B.
-
-(* ****DEPENDENCIES**** *)
-(* 
-#[repr(C)]
-#[derive(AlignedBorrow)]
+(*
 pub struct ImmInstruction<T> {
     pub is_valid: T,
-    /// Absolute opcode number
     pub opcode: T,
     pub immediate: T,
 }
 *)
 Module ImmInstruction.
-  Record t : Set := {
-    is_valid : Z;
-    op_code : Z;
-    immediate : Z;
+  Record t {T : Set} : Set := {
+    is_valid : T;
+    opcode : T;
+    immediate : T;
   }.
+  Arguments t : clear implicits.
+
+  Definition map {T1 T2 : Set} (f : T1 -> T2) (self : t T1) : t T2 := {|
+    ImmInstruction.is_valid := f self.(ImmInstruction.is_valid);
+    ImmInstruction.opcode := f self.(ImmInstruction.opcode);
+    ImmInstruction.immediate := f self.(ImmInstruction.immediate);
+  |}.
 End ImmInstruction.
 
-(* Inductive Expr : Set := | Make_Expr . *)
-(* Inductive BusIndex : Set := | Make_BusIndex . *)
-
-(* 
-pub struct Interaction<Expr> {
-    pub message: Vec<Expr>,
-    pub count: Expr,
-    /// The bus index specifying the bus to send the message over. All valid instantiations of
-    /// `BusIndex` are safe.
-    pub bus_index: BusIndex,
-    /// Determines the contribution of each interaction message to a linear constraint on the trace
-    /// heights in the verifier.
-    ///
-    /// For each bus index and trace, `count_weight` values are summed per interaction on that
-    /// bus index and multiplied by the trace height. The total sum over all traces is constrained
-    /// by the verifier to not overflow the field characteristic \( p \).
-    ///
-    /// This is used to impose sufficient conditions for bus constraint soundness and setting a
-    /// proper value depends on the bus and the constraint it imposes.
-    pub count_weight: u32,
-}
-*)
-
-(* Module Interaction.
-  Record t (e : Expr) : Set := {
-    message : list Expr;
-    count : Expr;
-    bus_index : BusIndex;
-    count_weight : Z;
-  }.
-End Interaction. *)
-
-(* NOTE: UNUSED *)
-Module VmAdapterInterface.
-  (* 
-  /// The interface between primitive AIR and machine adapter AIR.
-  pub trait VmAdapterInterface<T> {
-      /// The memory read data that should be exposed for downstream use
-      type Reads;
-      /// The memory write data that are expected to be provided by the integrator
-      type Writes;
-      /// The parts of the instruction that should be exposed to the integrator.
-      /// This will typically include `is_valid`, which indicates whether the trace row
-      /// is being used and `opcode` to indicate which opcode is being executed if the
-      /// VmChip supports multiple opcodes.
-      type ProcessedInstruction;
-  }
-  *)
-  Class t (T : Set) : Type := {
-    Reads : Set;
-    Writes : Set;
-    ProcessedInstruction : Set;
-  }.
-End VmAdapterInterface.
-
-(* 
+(*
 pub struct AdapterAirContext<T, I: VmAdapterInterface<T>> {
-    /// Leave as `None` to allow the adapter to decide the `to_pc` automatically.
-    pub to_pc: Option<T>,
-    pub reads: I::Reads,
-    pub writes: I::Writes,
-    pub instruction: I::ProcessedInstruction,
+  pub to_pc: Option<T>,
+  pub reads: I::Reads,
+  pub writes: I::Writes,
+  pub instruction: I::ProcessedInstruction,
 }
 *)
+(* TODO: move it to another file, as this is actually related to `integration_api.rs` *)
 Module AdapterAirContext.
-  Record t (instruction_type : Set) : Set := {
-    to_pc : option Z;
-    (* NOTE: for now we only design them as simple as they can be. We will
-    see how to extend them in the future *)
-    reads : list Z;
-    writes : list Z;
-    instruction : instruction_type;
+  Record t {NUM_LIMBS : Z} {T : Set} : Set := {
+    to_pc : option T;
+    (* I::Reads: From<[[AB::Expr; NUM_LIMBS]; 2]>, *)
+    reads : list (Array.t T NUM_LIMBS);
+    (* I::Writes: Default, *)
+    writes : list (Array.t T NUM_LIMBS);
+    (* I::ProcessedInstruction: From<ImmInstruction<AB::Expr>>, *)
+    instruction : ImmInstruction.t T;
+  }.
+  Arguments t : clear implicits.
+
+  Definition map {NUM_LIMBS : Z} {T1 T2 : Set} (f : T1 -> T2) (self : t NUM_LIMBS T1) :
+      t NUM_LIMBS T2 :=
+  {|
+    AdapterAirContext.to_pc := option_map f self.(AdapterAirContext.to_pc);
+    AdapterAirContext.reads := List.map (Array.map f) self.(AdapterAirContext.reads);
+    AdapterAirContext.writes := List.map (Array.map f) self.(AdapterAirContext.writes);
+    AdapterAirContext.instruction := ImmInstruction.map f self.(AdapterAirContext.instruction);
+  |}.
+
+  Global Instance AdapterAirContextIsEval {NUM_LIMBS : Z} {T : Set} `{Eval.C T Z} :
+      Eval.C (t NUM_LIMBS T) (t NUM_LIMBS Z) := {
+    eval p _ env self := map (Eval.eval env) self;
   }.
 End AdapterAirContext.
 
-(* 
-#[opcode_offset = 0x220]
-#[repr(usize)]
-#[allow(non_camel_case_types)]
+(* TODO: from `instructions.rs`, move there *)
+(*
 pub enum BranchEqualOpcode {
     BEQ,
     BNE,
 }
 *)
 Module BranchEqualOpcode.
-  Definition opcode_offset : Z := 0x220.
-
-  Inductive t :=
-  | BEQ
-  | BNE
-  .
-
-  Definition as_usize (x : t) : Z :=
-    match x with
-    | BEQ => Z.add 0 opcode_offset
-    | BNE => Z.add 1 opcode_offset
-    end.
-
-  Definition iter : list t := [BEQ; BNE].
+  Inductive t : Set :=
+    | BEQ
+    | BNE.
 End BranchEqualOpcode.
 
-(* 
-pub trait InteractionBuilder: AirBuilder {
-    /// Stores a new interaction in the builder.
-    ///
-    /// See [Interaction] for more details on `count_weight`.
-    fn push_interaction<E: Into<Self::Expr>>(
-        &mut self,
-        bus_index: BusIndex,
-        fields: impl IntoIterator<Item = E>,
-        count: impl Into<Self::Expr>,
-        count_weight: u32,
-    );
+(*
+pub struct BranchEqualCoreCols<T, const NUM_LIMBS: usize> {
+  pub a: [T; NUM_LIMBS],
+  pub b: [T; NUM_LIMBS],
 
-    /// Returns the current number of interactions.
-    fn num_interactions(&self) -> usize;
+  pub cmp_result: T,
+  pub imm: T,
 
-    /// Returns all interactions stored.
-    fn all_interactions(&self) -> &[Interaction<Self::Expr>];
+  pub opcode_beq_flag: T,
+  pub opcode_bne_flag: T,
+
+  pub diff_inv_marker: [T; NUM_LIMBS],
 }
 *)
-Module InteractionBuilder.
-  (* Datatype to present all asserted constraints from `assert_zero`, always and only *)
-  Module Assert.
-    Inductive t (A : Set) : Set :=
-      | Var : A -> t A
-      .
-    Arguments Var {_} _.
-  End Assert.
-
-  (* NOTE: for future reference
-  Class F {T : Type} : Type := {
-    get_num : Z;
+Module BranchEqualCoreCols.
+  Record t {NUM_LIMBS : Z} {T : Set} : Set := {
+    a : Array.t T NUM_LIMBS;
+    b : Array.t T NUM_LIMBS;
+    cmp_result : T;
+    imm : T;
+    opcode_beq_flag : T;
+    opcode_bne_flag : T;
+    diff_inv_marker : Array.t T NUM_LIMBS;
   }.
-  *)
-  Inductive F := 
-  | num_f : Z -> F.
+  Arguments t : clear implicits.
 
-  Inductive Var := 
-  | num_var : F -> Var.
+  Definition map {NUM_LIMBS : Z} {T1 T2 : Set} (f : T1 -> T2) (self : t NUM_LIMBS T1) :
+      t NUM_LIMBS T2 :=
+  {|
+    BranchEqualCoreCols.a := Array.map f self.(BranchEqualCoreCols.a);
+    BranchEqualCoreCols.b := Array.map f self.(BranchEqualCoreCols.b);
+    BranchEqualCoreCols.cmp_result := f self.(BranchEqualCoreCols.cmp_result);
+    BranchEqualCoreCols.imm := f self.(BranchEqualCoreCols.imm);
+    BranchEqualCoreCols.opcode_beq_flag := f self.(BranchEqualCoreCols.opcode_beq_flag);
+    BranchEqualCoreCols.opcode_bne_flag := f self.(BranchEqualCoreCols.opcode_bne_flag);
+    BranchEqualCoreCols.diff_inv_marker := Array.map f self.(BranchEqualCoreCols.diff_inv_marker);
+  |}.
 
-  Inductive Expr :=
-  | num_expr : Var -> Expr.
-
-  Definition M := list (list Var).
-
-  (* TODO: Extend to any types beyond Z in the future. The dependencies between 
-    the types seem to be a little bit hard to express. We might find some external way
-    to express this *)
-  Record Builder : Type := {
-    (* Types from AirBuilder
-    type F: Field;
-    type Expr: Algebra<Self::F> + Algebra<Self::Var>;
-    type Var: Into<Self::Expr>
-    type M: Matrix<Self::Var>;
-    *)
-    _F := F; 
-    _Expr := Expr;
-    _Var := Var;
-    _M := M;
-
-    (* Stores the context generated from `when` *)
-    constraints : list (Assert.t Expr);
-    (* Stores the result `assert_zero` makes *)
-    assertions : list (Assert.t Expr);
+  Global Instance map_mod {p} `{Prime p} {NUM_LIMBS : Z} : MapMod (t NUM_LIMBS Z) := {
+    map_mod := BranchEqualCoreCols.map map_mod;
   }.
-
-  Definition z_to_var (z : Z) : Var :=
-    num_var (num_f z).
-
-  Definition z_to_expr (z : Z) : Expr :=
-    num_expr (z_to_var z).
-
-  Definition f_to_z (f : F) : Z := let '(num_f n) := f in n.
-
-  Definition var_to_z (v : Var) : Z := let '(num_var f) := v in f_to_z f.
-
-  Definition expr_to_z (e : Expr) : Z := let '(num_expr v) := e in var_to_z v.
-
-  Definition assert_expr_to_z (a : Assert.t Expr) : Z :=
-    let '(Assert.Var x) := a in expr_to_z x.
-
-  (* NOTE: to be optimized *)
-  Fixpoint aggregate_constraints (l : list (Assert.t Expr)) : option (Assert.t Expr) :=
-    match l with
-    | x :: [] => Some x
-    | x :: xs => match (aggregate_constraints xs) with
-      | Some x' => 
-        let x := assert_expr_to_z x in
-        let x' := assert_expr_to_z x' in
-        Some (Assert.Var (z_to_expr (Z.mul x x')))
-      | None => None
-      end
-    | [] => None
-    end.
-
-  Definition when (builder : Builder) (c : Assert.t builder.(_Expr)) : Builder :=
-    let c' := builder.(constraints) in
-    let a' := builder.(assertions) in
-    Build_Builder (c :: c') a'.
-  
-  (* Pop a constraint off to simulate one constraint being removed. When it comes to 
-  monad, a structure similar tos a stack would be helpful *)
-  Definition end_when (builder : Builder) : Builder :=
-    let c' := builder.(constraints) in
-    let c := match c' with
-    | [] => c'
-    | _ :: c => c
-    end in
-    let a' := builder.(assertions) in
-    Build_Builder c a'.
-  
-  (* NOTE: every other primitives are built on this primitive *)
-  Definition assert_zero (builder : Builder) 
-    (e : builder.(_Expr)) : Builder :=
-    let c' := builder.(constraints) in
-    let a := aggregate_constraints (c' ++ [Assert.Var e]) in
-    (* desugar the option *)
-    let a := match a with
-    | Some a' => a'
-    | None => Assert.Var e
-    end in
-    let '(Assert.Var a) := a in
-    let a := if Z.eqb 0 (expr_to_z a) then 1%Z else 0%Z in
-    Build_Builder c' (builder.(assertions) ++ [Assert.Var (z_to_expr a)]).
-
-  Definition assert_one (builder : Builder) (e : builder.(_Expr)) : Builder :=
-    let z := expr_to_z e in
-    assert_zero builder (z_to_expr (Z.sub 1 z)).
-
-  Definition assert_bool (builder : Builder) (e : builder.(_Expr)) : Builder :=
-    let z := expr_to_z e in
-    let bool_check := Z.mul z (Z.sub 1%Z z) in
-    assert_zero builder (z_to_expr bool_check).
-End InteractionBuilder.
-
-(* NOTE: for reference
-#[proc_macro_derive(AlignedBorrow)]
-pub fn aligned_borrow_derive(input: TokenStream) -> TokenStream {
-    let ast = parse_macro_input!(input as DeriveInput);
-    let name = &ast.ident;
-
-    // Get first generic which must be type (ex. `T`) for input <T, N: NumLimbs, const M: usize>
-    let type_generic = ast
-        .generics
-        .params
-        .iter()
-        .map(|param| match param {
-            GenericParam::Type(type_param) => &type_param.ident,
-            _ => panic!("Expected first generic to be a type"),
-        })
-        .next()
-        .expect("Expected at least one generic");
-
-    // Get generics after the first (ex. `N: NumLimbs, const M: usize`)
-    // We need this because when we assert the size, we want to substitute u8 for T.
-    let non_first_generics = ast
-        .generics
-        .params
-        .iter()
-        .skip(1)
-        .filter_map(|param| match param {
-            GenericParam::Type(type_param) => Some(&type_param.ident),
-            GenericParam::Const(const_param) => Some(&const_param.ident),
-            _ => None,
-        })
-        .collect::<Vec<_>>();
-
-    // Get impl generics (`<T, N: NumLimbs, const M: usize>`), type generics (`<T, N>`), where
-    // clause (`where T: Clone`)
-    let (impl_generics, type_generics, where_clause) = ast.generics.split_for_impl();
-
-    impl #impl_generics core::borrow::Borrow<#name #type_generics> for [#type_generic] #where_clause {
-        fn borrow(&self) -> &#name #type_generics {
-            debug_assert_eq!(self.len(), #name::#type_generics::width());
-            let (prefix, shorts, _suffix) = unsafe { self.align_to::<#name #type_generics>() };
-            debug_assert!(prefix.is_empty(), "Alignment should match");
-            debug_assert_eq!(shorts.len(), 1);
-            &shorts[0]
-        }
-    }
-
-
-    let methods = quote! {
-        impl #impl_generics core::borrow::Borrow<#name #type_generics> for [#type_generic] #where_clause {
-            fn borrow(&self) -> &#name #type_generics {
-                debug_assert_eq!(self.len(), #name::#type_generics::width());
-                let (prefix, shorts, _suffix) = unsafe { self.align_to::<#name #type_generics>() };
-                debug_assert!(prefix.is_empty(), "Alignment should match");
-                debug_assert_eq!(shorts.len(), 1);
-                &shorts[0]
-            }
-        }
-
-        impl #impl_generics core::borrow::BorrowMut<#name #type_generics> for [#type_generic] #where_clause {
-            fn borrow_mut(&mut self) -> &mut #name #type_generics {
-                debug_assert_eq!(self.len(), #name::#type_generics::width());
-                let (prefix, shorts, _suffix) = unsafe { self.align_to_mut::<#name #type_generics>() };
-                debug_assert!(prefix.is_empty(), "Alignment should match");
-                debug_assert_eq!(shorts.len(), 1);
-                &mut shorts[0]
-            }
-        }
-
-        impl #impl_generics #name #type_generics {
-            pub const fn width() -> usize {
-                std::mem::size_of::<#name<u8 #(, #non_first_generics)*>>()
-            }
-        }
-    };
-
-    TokenStream::from(methods)
-}
-*)
-
-(* *************************** *)
-(* ****END OF DEPENDENCIES**** *)
-(* *************************** *)
+End BranchEqualCoreCols.
 
 (*
-#[repr(C)]
-#[derive(AlignedBorrow)]
-pub struct BranchEqualCoreCols<T, const NUM_LIMBS: usize> {
-    pub a: [T; NUM_LIMBS],
-    pub b: [T; NUM_LIMBS],
-
-    // Boolean result of a op b. Should branch if and only if cmp_result = 1.
-    pub cmp_result: T,
-    pub imm: T,
-
-    pub opcode_beq_flag: T,
-    pub opcode_bne_flag: T,
-
-    pub diff_inv_marker: [T; NUM_LIMBS],
-}
-*)
-(* For similar reason to above, here we put in a concrete type and later we will
-see how to extend the type *)
-(* NOTE that we didnt use the T here... *)
-Record BranchEqualCoreCols (NUM_LIMBS : Z) : Set := {
-  a : list InteractionBuilder.Expr;
-  b : list InteractionBuilder.Expr;
-  cmp_result : InteractionBuilder.Expr;
-  imm : InteractionBuilder.Expr;
-  opcode_beq_flag : InteractionBuilder.Expr;
-  opcode_bne_flag : InteractionBuilder.Expr;
-  diff_inv_marker : list InteractionBuilder.Expr;
-}.
-
-(* From #[derive(AlignedBorrow)]
-impl <T NUM_LIMBS> core::borrow::Borrow<BranchEqualCoreCols T NUM_LIMBS> for [T] {
-    fn borrow(&self) -> &BranchEqualCoreCols T NUM_LIMBS {
-        debug_assert_eq!(self.len(), BranchEqualCoreCols::<T NUM_LIMBS>::width());
-        let (prefix, shorts, _suffix) = unsafe { self.align_to::<BranchEqualCoreCols T NUM_LIMBS>() };
-        debug_assert!(prefix.is_empty(), "Alignment should match");
-        debug_assert_eq!(shorts.len(), 1);
-        &shorts[0]
-    }
-}
-*)
-Module Impl_Borrow_BranchEqualCoreCols_for_T.
-  Fixpoint next_helper {T : Set} (n : nat) (src : list T) (store : list T) : list T * list T :=
-    match n with
-    | O => (src, store)
-    | S n' => match src with
-      | x :: xs => next_helper n' xs (store ++ [x])
-      | [] => (src, store)
-      end
-    end.
-
-  (* slice the first n elements of a list, return it with the remaining part of the list *)
-  Definition next {T : Set} (n : nat) (src : list T) : list T * list T :=
-    next_helper n src [].
-
-  (* NOTE: for now, InteractionBuilder only *)
-  Definition borrow (cols : list InteractionBuilder.Var) (NUM_LIMBS : Z) (default_T : InteractionBuilder.Var)
-    : BranchEqualCoreCols NUM_LIMBS :=
-    let NUM_LIMBS' := Z.to_nat NUM_LIMBS in
-    let (cols, a) := next NUM_LIMBS' cols in
-    let a := map InteractionBuilder.num_expr a in
-    let (cols, b) := next NUM_LIMBS' cols in
-    let b := map InteractionBuilder.num_expr b in
-    let (cols, cmp_result) := next 1 cols in
-    let cmp_result := InteractionBuilder.num_expr (match (head cmp_result) with | Some x => x | None => default_T end) in
-    let (cols, imm) := next 1 cols in
-    let imm := InteractionBuilder.num_expr (match (head imm) with | Some x => x | None => default_T end) in
-    let (cols, opcode_beq_flag) := next 1 cols in
-    let opcode_beq_flag := InteractionBuilder.num_expr (match (head opcode_beq_flag) with | Some x => x | None => default_T end) in
-    let (cols, opcode_bne_flag) := next 1 cols in
-    let opcode_bne_flag := InteractionBuilder.num_expr (match (head opcode_bne_flag) with | Some x => x | None => default_T end) in
-    let (cols, diff_inv_marker) := next NUM_LIMBS' cols in
-    let diff_inv_marker := map InteractionBuilder.num_expr diff_inv_marker in
-    Build_BranchEqualCoreCols NUM_LIMBS
-      a b cmp_result imm opcode_beq_flag opcode_bne_flag diff_inv_marker.
-End Impl_Borrow_BranchEqualCoreCols_for_T.
-
-(* 
-#[derive(Copy, Clone, Debug)]
 pub struct BranchEqualCoreAir<const NUM_LIMBS: usize> {
-    offset: usize,
-    pc_step: u32,
+  offset: usize,
+  pc_step: u32,
 }
 *)
 Module BranchEqualCoreAir.
-  Record t (NUM_LIMBS : Z) : Set := {
+  Record t {NUM_LIMBS : Z} : Set := {
     offset : Z;
     pc_step : Z;
   }.
+  Arguments t : clear implicits.
 End BranchEqualCoreAir.
 
-(* 
-impl<F: Field, const NUM_LIMBS: usize> BaseAir<F> for BranchEqualCoreAir<NUM_LIMBS> {
-    fn width(&self) -> usize {
-        BranchEqualCoreCols::<F, NUM_LIMBS>::width()
-    }
-}
-*)
-Module Impl_BaseAir_for_BranchEqualCoreAir.
-(* TODO: investigate the macro to get the exact meaning *)
-(* 
-  pub const fn width() -> usize {
-      std::mem::size_of::<#name<u8 #(, #non_first_generics)*>>()
-  }
-*)
-End Impl_BaseAir_for_BranchEqualCoreAir.
+Fixpoint sum_for_in_zero_to_n_starting_from_aux {p} `{Prime p} (n : nat) (f : Z -> Z) (start : Z) :
+    Z :=
+  match n with
+  | O => start
+  | S n => BinOp.add (sum_for_in_zero_to_n_starting_from_aux n f start) (f (Z.of_nat n))
+  end.
 
-(* 
-impl<F: Field, const NUM_LIMBS: usize> BaseAirWithPublicValues<F>
-    for BranchEqualCoreAir<NUM_LIMBS>
-{
-}
-*)
-Module Impl_BaseAirWithPublicValues_for_BranchEqualCoreAir.
-  (* NOTE: BaseAirWithPublicValues should be able to use all functions from
-   BranchEqualCoreAir *)
-End Impl_BaseAirWithPublicValues_for_BranchEqualCoreAir.
+Definition sum_for_in_zero_to_n_starting_from {p} `{Prime p} (n : Z) (f : Z -> Z) (start : Z) : Z :=
+  sum_for_in_zero_to_n_starting_from_aux (Z.to_nat n) f start.
 
-(* 
-impl<AB, I, const NUM_LIMBS: usize> VmCoreAir<AB, I> for BranchEqualCoreAir<NUM_LIMBS>
-where
-    AB: InteractionBuilder,
-    I: VmAdapterInterface<AB::Expr>,
-    I::Reads: From<[[AB::Expr; NUM_LIMBS]; 2]>,
-    I::Writes: Default,
-    I::ProcessedInstruction: From<ImmInstruction<AB::Expr>>,
-{
-*)
-Module Impl_VmCoreAir_for_BranchEqualCoreAir.
-  Section Impl.
-  Import InteractionBuilder.
-  Import Number.
+Definition eval {p} `{Prime p} {NUM_LIMBS : Z}
+    (self : BranchEqualCoreAir.t NUM_LIMBS)
+    (local : BranchEqualCoreCols.t NUM_LIMBS Z)
+    (from_pc : Z) :
+    M.t (AdapterAirContext.t NUM_LIMBS Z) :=
+  let flags : list Z := [
+    local.(BranchEqualCoreCols.opcode_beq_flag);
+    local.(BranchEqualCoreCols.opcode_bne_flag)
+  ] in
 
-  Context (builder : InteractionBuilder.Builder). (* We ignore the AB for now *)
-  (* Context `{I : VmAdapterInterface.t}. *)
-  (* NOTE: I stands for a `AdapterInterface` type being used in other places
-  Demo to require subfield of I to be instance:
-  Context `{From I.Reads}. *)
-  Variable NUM_LIMBS : Z.
+  let* is_valid : Z :=
+    M.List.fold_left
+      (fun acc flag =>
+        let* _ := M.assert_bool flag in
+        M.pure (BinOp.add acc flag)
+      )
+      Z.zero
+      flags in
+  let* _ := M.assert_bool is_valid in
+  let* _ := M.assert_bool local.(BranchEqualCoreCols.cmp_result) in
 
-  Definition Self := BranchEqualCoreAir.t NUM_LIMBS.
+  let a : Array.t Z NUM_LIMBS := local.(BranchEqualCoreCols.a) in
+  let b : Array.t Z NUM_LIMBS := local.(BranchEqualCoreCols.b) in
+  let inv_marker : Array.t Z NUM_LIMBS := local.(BranchEqualCoreCols.diff_inv_marker) in
 
-  Parameter default_AB_Var : builder.(_Var).
-  Parameter default_AB_Expr : builder.(_Expr).
-
-  (* ********FUNCTIIONS******** *)
-  (* 
-  fn eval(
-          &self,
-          builder: &mut AB,
-          local: &[AB::Var],
-          from_pc: AB::Var,
-      ) -> AdapterAirContext<AB::Expr, I> {
-  *)
-  (* NOTE: In this function:
-  - `record` collects all constraints, which is the primary goal for current implementation
-  *)
-  Definition eval 
-    (self : Self) 
-    (local : list builder.(_Var)) (from_pc : builder.(_Var)) : 
-      (@RecordRun (AdapterAirContext.t ImmInstruction.t) Builder) :=
-    (* 
-    let cols: &BranchEqualCoreCols<_, NUM_LIMBS> = local.borrow();
-    let flags = [cols.opcode_beq_flag, cols.opcode_bne_flag];
-    *)
-    let cols := @Impl_Borrow_BranchEqualCoreCols_for_T.borrow
-      local NUM_LIMBS default_AB_Var in
-    let f1 := cols.(opcode_beq_flag NUM_LIMBS) in
-    let f2 := cols.(opcode_bne_flag NUM_LIMBS) in
-    (* 
-    let is_valid = flags.iter().fold(AB::Expr::ZERO, |acc, &flag| {
-              builder.assert_bool(flag);
-              acc + flag.into()
-          });
-    *)
-    let builder := assert_bool builder f1 in
-    let builder := assert_bool builder f2 in
-    let is_valid := Z.add (InteractionBuilder.expr_to_z f1) (InteractionBuilder.expr_to_z f2) in
-    let is_valid_expr := InteractionBuilder.z_to_expr is_valid in
-    (* 
-    builder.assert_bool(is_valid.clone());
-    builder.assert_bool(cols.cmp_result);
-    *)
-    let builder := assert_bool builder is_valid_expr in
-    let cmp_result_expr := cols.(cmp_result NUM_LIMBS) in
-    let cmp_result := InteractionBuilder.expr_to_z cmp_result_expr in
-    let builder := assert_bool builder cmp_result_expr in
-    (* 
-    let a = &cols.a;
-    let b = &cols.b;
-    let inv_marker = &cols.diff_inv_marker;
-    *)
-    let a := cols.(a NUM_LIMBS) in
-    let b := cols.(b NUM_LIMBS) in
-    let inv_maker := cols.(diff_inv_marker NUM_LIMBS) in
-    (* 
-    // 1 if cmp_result indicates a and b are equal, 0 otherwise
-    let cmp_eq =
-        cols.cmp_result * cols.opcode_beq_flag + not(cols.cmp_result) * cols.opcode_bne_flag;
-    let mut sum = cmp_eq.clone();
-    *)
-    let opcode_beq_flag_expr := cols.(opcode_beq_flag NUM_LIMBS) in
-    let opcode_beq_flag := InteractionBuilder.expr_to_z opcode_beq_flag_expr in
-    let opcode_bne_flag_expr := cols.(opcode_bne_flag NUM_LIMBS) in
-    let opcode_bne_flag := InteractionBuilder.expr_to_z opcode_bne_flag_expr in
-    let cmp_eq := Z.add (Z.mul cmp_result opcode_beq_flag)
-      (Z.mul (Z.sub 1 cmp_result) opcode_bne_flag) in
-    let sum := cmp_eq in
-    (* 
-    // For BEQ, inv_marker is used to check equality of a and b:
-    // - If a == b, all inv_marker values must be 0 (sum = 0)
-    // - If a != b, inv_marker contains 0s for all positions except ONE position i where a[i] !=
-    //   b[i]
-    // - At this position, inv_marker[i] contains the multiplicative inverse of (a[i] - b[i])
-    // - This ensures inv_marker[i] * (a[i] - b[i]) = 1, making the sum = 1
-    // Note: There might be multiple valid inv_marker if a != b.
-    // But as long as the trace can provide at least one, that’s sufficient to prove a != b.
-    //
-    // Note:
-    // - If cmp_eq == 0, then it is impossible to have sum != 0 if a == b.
-    // - If cmp_eq == 1, then it is impossible for a[i] - b[i] == 0 to pass for all i if a != b.
-    for i in 0..NUM_LIMBS {
-        sum += (a[i] - b[i]) * inv_marker[i];
-        builder.assert_zero(cmp_eq.clone() * (a[i] - b[i]));
-    }
-    builder.when(is_valid.clone()).assert_one(sum); 
-    *)
-    (* NOTE: A sole line `when(a).b` works as just a * b. If a sub builder 
-      is built with `when`, every constraints for the sub builder are prefixed with `a *`.
-    *)
-    let fix loop (n : nat) (sum : Z) 
-      (builder : Builder) {struct n} := 
-      match n with 
-      | O => (sum, builder)
-      | S n' =>
-        (* 0 <= x < NUM_LIMBS *)
-        let x := minus (minus (Z.to_nat NUM_LIMBS) 1) n' in
-        let a_i := InteractionBuilder.expr_to_z (nth x a default_AB_Expr) in
-        let b_i := InteractionBuilder.expr_to_z (nth x b default_AB_Expr) in
-        let inv_maker_i := InteractionBuilder.expr_to_z 
-          (nth x inv_maker default_AB_Expr) in
-        let sum := Z.add sum (Z.mul (Z.sub a_i b_i) inv_maker_i) in
-        let builder := assert_zero builder 
-          (InteractionBuilder.z_to_expr (Z.mul cmp_eq (Z.sub a_i b_i))) in
-        loop n' sum builder
-      end
-    in
-    let (sum, builder) := loop (Z.to_nat NUM_LIMBS) sum builder in
-    let builder := when builder (Assert.Var is_valid_expr) in
-    let builder := assert_one builder (InteractionBuilder.z_to_expr sum) in 
-    let builder := end_when builder in
-    (* 
-    let expected_opcode = flags
-        .iter()
-        .zip(BranchEqualOpcode::iter())
-        .fold(AB::Expr::ZERO, |acc, (flag, opcode)| {
-            acc + ( \*flag).into() * AB::Expr::from_canonical_u8(opcode as u8)
-        })
-        + AB::Expr::from_canonical_usize(self.offset);
-    *)
-    (* NOTE: WARNING: 
-    - We dont't check the boundary for u8
-    - The computation here is being completed immediately. Maybe we should also do it 
-      for other computations. Same for the code blocks followed 
-    *)
-    let opcodes := map BranchEqualOpcode.as_usize BranchEqualOpcode.iter in
-    let o1 := nth 0 opcodes BranchEqualOpcode.opcode_offset in
-    let o2 := nth 1 opcodes BranchEqualOpcode.opcode_offset in
-    let expected_opcode := Z.add 
-      (Z.mul (InteractionBuilder.expr_to_z f1) o1) (Z.mul (InteractionBuilder.expr_to_z f2) o2) in
-    (* 
-    let to_pc = from_pc
-              + cols.cmp_result * cols.imm
-              + not(cols.cmp_result) * AB::Expr::from_canonical_u32(self.pc_step);
-    *)
-    let to_pc := InteractionBuilder.var_to_z from_pc in
-    let imm := InteractionBuilder.expr_to_z (cols.(imm NUM_LIMBS)) in
-    let to_pc := Z.add to_pc (Z.mul cmp_result imm) in
-    let pc_step := self.(BranchEqualCoreAir.pc_step NUM_LIMBS) in
-    let to_pc := Z.add to_pc (Z.mul (Z.sub 1 cmp_result) pc_step) in
-    (* 
-    AdapterAirContext {
-        to_pc: Some(to_pc),
-        reads: [cols.a.map(Into::into), cols.b.map(Into::into)].into(),
-        writes: Default::default(),
-        instruction: ImmInstruction {
-            is_valid,
-            opcode: expected_opcode,
-            immediate: cols.imm.into(),
-        }
-        .into(),
-    }
-    *)
-    let a := map InteractionBuilder.expr_to_z a in
-    let b := map InteractionBuilder.expr_to_z b in
-    let reads := a ++ b in
-    let context := (AdapterAirContext.Build_t ImmInstruction.t
-      (Some to_pc) reads []
-      (ImmInstruction.Build_t is_valid expected_opcode imm)
+  let* cmp_eq : Z :=
+    M.pure (
+      BinOp.add
+        (BinOp.mul local.(BranchEqualCoreCols.cmp_result) local.(BranchEqualCoreCols.opcode_beq_flag))
+        (BinOp.mul (M.not local.(BranchEqualCoreCols.cmp_result)) local.(BranchEqualCoreCols.opcode_bne_flag))
     ) in
-    (context, builder).
-  End Impl.
-End Impl_VmCoreAir_for_BranchEqualCoreAir.
 
-Module _Test.
-Definition builder : InteractionBuilder.Builder := InteractionBuilder.Build_Builder [] [].
+  let* _ := M.for_in_zero_to_n NUM_LIMBS (fun i =>
+    M.assert_zero (BinOp.mul cmp_eq (BinOp.sub (Array.get a i) (Array.get b i)))
+  ) in
+  let sum : Z := sum_for_in_zero_to_n_starting_from NUM_LIMBS (fun i =>
+    BinOp.mul (BinOp.sub (Array.get a i) (Array.get b i)) (Array.get inv_marker i)
+  ) cmp_eq in
+  let* _ := M.when is_valid (M.assert_one sum) in
 
-Definition NUM_LIMBS : Z := 8.
+  let flags_with_opcode_integer : list (Z * Z) :=
+    [
+      (local.(BranchEqualCoreCols.opcode_beq_flag), 0);
+      (local.(BranchEqualCoreCols.opcode_bne_flag), 1)
+    ] in
+  let expected_opcode : Z :=
+    Lists.List.fold_left
+      (fun acc '(flag, opcode) =>
+        BinOp.add acc (BinOp.mul flag opcode)
+      )
+      flags_with_opcode_integer
+      0 in
+  let expected_opcode : Z :=
+    BinOp.add expected_opcode self.(BranchEqualCoreAir.offset) in
 
-Definition a := map Z.of_nat [0; 0; 0; 0; 0; 0; 0; 0].
-Definition b := map Z.of_nat [0; 0; 0; 0; 0; 0; 0; 0].
+  let to_pc : Z :=
+    BinOp.add
+      (BinOp.add
+        from_pc
+        (BinOp.mul local.(BranchEqualCoreCols.cmp_result) local.(BranchEqualCoreCols.imm))
+      )
+      (BinOp.mul (M.not local.(BranchEqualCoreCols.cmp_result)) self.(BranchEqualCoreAir.pc_step))
+    in
 
-Definition cmp_result := 1%Z.
-Definition imm := 1%Z.
-Definition opcode_beq_flag := 1%Z.
-Definition opcode_bne_flag := 1%Z.
-Definition diff_inv_marker := map Z.of_nat [0; 0; 0; 0; 0; 0; 0; 0].
-
-Definition local : list InteractionBuilder.Var :=
-  let stream := a ++ b ++ [cmp_result; imm; opcode_beq_flag; opcode_bne_flag ] ++ diff_inv_marker in
-  map InteractionBuilder.z_to_var stream.
-
-Definition from_pc : InteractionBuilder.Var := InteractionBuilder.z_to_var 0%Z.
-
-Definition self : BranchEqualCoreAir.t NUM_LIMBS := BranchEqualCoreAir.Build_t NUM_LIMBS 0%Z 4%Z.
-
-Definition result := Impl_VmCoreAir_for_BranchEqualCoreAir.eval builder NUM_LIMBS self local from_pc.
-
-Definition result_builder := let '(_, b) := result in b.
-
-Definition builder_assertions := result_builder.(InteractionBuilder.assertions).
-
-End _Test.
-
-
-(*
-    fn start_offset(&self) -> usize {
-        self.offset
-    }
-}
-
-#[repr(C)]
-#[derive(Clone, Debug, Serialize, Deserialize)]
-pub struct BranchEqualCoreRecord<T, const NUM_LIMBS: usize> {
-    #[serde(with = "BigArray")]
-    pub a: [T; NUM_LIMBS],
-    #[serde(with = "BigArray")]
-    pub b: [T; NUM_LIMBS],
-    pub cmp_result: T,
-    pub imm: T,
-    pub diff_inv_val: T,
-    pub diff_idx: usize,
-    pub opcode: BranchEqualOpcode,
-}
-
-#[derive(Debug)]
-pub struct BranchEqualCoreChip<const NUM_LIMBS: usize> {
-    pub air: BranchEqualCoreAir<NUM_LIMBS>,
-}
-
-impl<const NUM_LIMBS: usize> BranchEqualCoreChip<NUM_LIMBS> {
-    pub fn new(offset: usize, pc_step: u32) -> Self {
-        Self {
-            air: BranchEqualCoreAir { offset, pc_step },
-        }
-    }
-}
-
-impl<F: PrimeField32, I: VmAdapterInterface<F>, const NUM_LIMBS: usize> VmCoreChip<F, I>
-    for BranchEqualCoreChip<NUM_LIMBS>
-where
-    I::Reads: Into<[[F; NUM_LIMBS]; 2]>,
-    I::Writes: Default,
-{
-    type Record = BranchEqualCoreRecord<F, NUM_LIMBS>;
-    type Air = BranchEqualCoreAir<NUM_LIMBS>;
-
-    #[allow(clippy::type_complexity)]
-    fn execute_instruction(
-        &self,
-        instruction: &Instruction<F>,
-        from_pc: u32,
-        reads: I::Reads,
-    ) -> Result<(AdapterRuntimeContext<F, I>, Self::Record)> {
-        let Instruction { opcode, c: imm, .. } = *instruction;
-        let branch_eq_opcode =
-            BranchEqualOpcode::from_usize(opcode.local_opcode_idx(self.air.offset));
-
-        let data: [[F; NUM_LIMBS]; 2] = reads.into();
-        let x = data[0].map(|x| x.as_canonical_u32());
-        let y = data[1].map(|y| y.as_canonical_u32());
-        let (cmp_result, diff_idx, diff_inv_val) = run_eq::<F, NUM_LIMBS>(branch_eq_opcode, &x, &y);
-
-        let output = AdapterRuntimeContext {
-            to_pc: cmp_result.then_some((F::from_canonical_u32(from_pc) + imm).as_canonical_u32()),
-            writes: Default::default(),
-        };
-        let record = BranchEqualCoreRecord {
-            opcode: branch_eq_opcode,
-            a: data[0],
-            b: data[1],
-            cmp_result: F::from_bool(cmp_result),
-            imm,
-            diff_idx,
-            diff_inv_val,
-        };
-
-        Ok((output, record))
-    }
-
-    fn get_opcode_name(&self, opcode: usize) -> String {
-        format!(
-            "{:?}",
-            BranchEqualOpcode::from_usize(opcode - self.air.offset)
-        )
-    }
-
-    fn generate_trace_row(&self, row_slice: &mut [F], record: Self::Record) {
-        let row_slice: &mut BranchEqualCoreCols<_, NUM_LIMBS> = row_slice.borrow_mut();
-        row_slice.a = record.a;
-        row_slice.b = record.b;
-        row_slice.cmp_result = record.cmp_result;
-        row_slice.imm = record.imm;
-        row_slice.opcode_beq_flag = F::from_bool(record.opcode == BranchEqualOpcode::BEQ);
-        row_slice.opcode_bne_flag = F::from_bool(record.opcode == BranchEqualOpcode::BNE);
-        row_slice.diff_inv_marker = array::from_fn(|i| {
-            if i == record.diff_idx {
-                record.diff_inv_val
-            } else {
-                F::ZERO
-            }
-        });
-    }
-
-    fn air(&self) -> &Self::Air {
-        &self.air
-    }
-}
-
-// Returns (cmp_result, diff_idx, x[diff_idx] - y[diff_idx])
-pub(super) fn run_eq<F: PrimeField32, const NUM_LIMBS: usize>(
-    local_opcode: BranchEqualOpcode,
-    x: &[u32; NUM_LIMBS],
-    y: &[u32; NUM_LIMBS],
-) -> (bool, usize, F) {
-    for i in 0..NUM_LIMBS {
-        if x[i] != y[i] {
-            return (
-                local_opcode == BranchEqualOpcode::BNE,
-                i,
-                (F::from_canonical_u32(x[i]) - F::from_canonical_u32(y[i])).inverse(),
-            );
-        }
-    }
-    (local_opcode == BranchEqualOpcode::BEQ, 0, F::ZERO)
-}
-*)
+  M.pure {|
+    AdapterAirContext.to_pc := Some to_pc;
+    AdapterAirContext.reads := [a; b];
+    AdapterAirContext.writes := [];
+    AdapterAirContext.instruction := {|
+      ImmInstruction.is_valid := is_valid;
+      ImmInstruction.opcode := expected_opcode;
+      ImmInstruction.immediate := local.(BranchEqualCoreCols.imm);
+    |};
+  |}.
